Attempt to remove dependent types in bitvectors (some proofs needs to be reworked)

src/SMT_terms.v
@@ -13,6 +13,7 @@
 (*                                                                        *)
 (**************************************************************************)
 
+(* Add Rec LoadPath "." as SMTCoq. *)
 
 Require Import Bool Int63 PArray.
 (*Add LoadPath "/home/burak/Desktop/smtcoq/src/bva".*)
@@ -69,7 +70,7 @@ Module Form.
 
   Section Interp.
     Variable interp_atom : atom -> bool.
-    Variable interp_bvatom : atom -> forall s, BITVECTOR_LIST.bitvector s.
+    Variable interp_bvatom : atom -> BITVECTOR_LIST.bitvector.
 
     Section Interp_form.
 
@@ -97,7 +98,7 @@ Module Form.
         | FbbT a ls =>
           let ils := List.map (Lit.interp interp_var) ls in
           let n := N.of_nat (List.length ils) in
-          BITVECTOR_LIST.bv_eq (interp_bvatom a n) (BITVECTOR_LIST.of_bits ils)
+          BITVECTOR_LIST.bv_eq (interp_bvatom a) (BITVECTOR_LIST.of_bits ils)
         end.
 
     End Interp_form.
@@ -305,7 +306,7 @@ Module Typ.
   | TZ : type
   | Tbool : type
   | Tpositive : type
-  | TBV : N -> type.
+  | TBV : type.
 
   Definition ftype := (list type * type)%type.
 
@@ -319,7 +320,7 @@ Module Typ.
       | TZ => Z
       | Tbool => bool
       | Tpositive => positive
-      | TBV n => BITVECTOR_LIST.bitvector n
+      | TBV => BITVECTOR_LIST.bitvector
       end.
 
     Definition interp_ftype (t:ftype) :=
@@ -335,7 +336,7 @@ Module Typ.
         | TZ => Zeq_bool
         | Tbool => Bool.eqb
         | Tpositive => Peqb
-        | TBV n => @BITVECTOR_LIST.bv_eq n
+        | TBV => @BITVECTOR_LIST.bv_eq
         end.
 
       Lemma i_eqb_spec : forall t x y, i_eqb t x y <-> x = y.
@@ -345,7 +346,10 @@ Module Typ.
        symmetry;apply Zeq_is_eq_bool.
        apply Bool.eqb_true_iff.
        apply Peqb_eq.
+       split.
        apply BITVECTOR_LIST.bv_eq_reflect.
+       intro. rewrite H. 
+       apply BITVECTOR_LIST.bv_eq_reflect. easy.
       Qed.
 
       Lemma reflect_i_eqb : forall t x y, reflect (x = y) (i_eqb t x y).
@@ -425,11 +429,11 @@ Module Typ.
       | TZ, TZ => idcast
       | Tbool, Tbool => idcast
       | Tpositive, Tpositive => idcast
-      | TBV n, TBV m =>
-        match N_cast n m with
-        | Some k => Cast (fun P => k (fun y => P (TBV y)))
-        | None => NoCast
-        end
+      | TBV, TBV => idcast
+        (* match N_cast n m with *)
+        (* | Some k => Cast (fun P => k (fun y => P (TBV y))) *)
+        (* | None => NoCast *)
+        (* end *)
       | _, _ => NoCast
       end.
 
@@ -446,7 +450,7 @@ Module Typ.
     Proof.
       intros A0;destruct A0;simpl;trivial.
       rewrite cast_refl;trivial.
-      rewrite N_cast_refl;trivial.
+      (* rewrite N_cast_refl;trivial. *)
     Qed.
 
     (* Remark : I use this definition because eqb will not be used only in the interpretation *)
@@ -456,7 +460,7 @@ Module Typ.
       | TZ, TZ => true
       | Tbool, Tbool => true
       | Tpositive, Tpositive => true
-      | TBV n, TBV m => N.eqb n m
+      | TBV, TBV => true
       | _,_ => false
       end.
 
@@ -495,7 +499,7 @@ Module Typ.
     Proof.
       intros A0 B0;destruct A0; destruct B0;simpl;trivial;try discriminate.
       intros Heq;rewrite (cast_diff _ _ Heq);trivial.
-      rewrite N.eqb_neq. intro Heq. now rewrite N_cast_diff.
+      (* rewrite N.eqb_neq. intro Heq. now rewrite N_cast_diff. *)
     Qed.
 
     Lemma neq_cast : forall A B,
@@ -508,12 +512,15 @@ Module Typ.
     Proof.
       intros x y; destruct x;destruct y;simpl;try constructor;trivial;try discriminate.
       apply iff_reflect;rewrite eqb_spec;split;intros H;[inversion H | subst]; trivial.
-      apply iff_reflect. rewrite N.eqb_eq. split;intros H;[inversion H | subst]; trivial.
+      (* apply iff_reflect. rewrite N.eqb_eq. split;intros H;[inversion H | subst]; trivial. *)
     Qed.
 
     Lemma eqb_spec : forall x y, eqb x y <-> x = y.
     Proof.
-      intros;symmetry;apply reflect_iff;apply reflect_eqb.
+      intros.
+      symmetry.
+      apply reflect_iff.
+      apply reflect_eqb.
     Qed.
 
     Lemma eqb_refl : forall x, eqb x x.
@@ -593,12 +600,13 @@ Module Atom.
    | BO_Zgt
    | BO_eq (_ : Typ.type)
    | BO_BVand (_: N)
-   | BO_BVor (_: N)
-   | BO_BVxor (_: N)
-   | BO_BVadd (_: N)
-   | BO_BVsubst (_: N)
-   | BO_BVmult (_: N).
-
+   (* | BO_BVor (_: N) *)
+   (* | BO_BVxor (_: N) *)
+   (* | BO_BVadd (_: N) *)
+   (* | BO_BVsubst (_: N) *)
+   (* | BO_BVmult (_: N) *)
+  .
+  
   Inductive nop : Type :=
    | NO_distinct (_ : Typ.type).
 
@@ -644,12 +652,12 @@ Module Atom.
    | BO_Zge, BO_Zge
    | BO_Zgt, BO_Zgt => true
    | BO_eq t, BO_eq t' => Typ.eqb t t'
-   | BO_BVand s1, BO_BVand s2
-   | BO_BVor s1, BO_BVor s2 
-   | BO_BVxor s1, BO_BVxor s2
-   | BO_BVadd s1, BO_BVadd s2 
-   | BO_BVsubst s1, BO_BVsubst s2 
-   | BO_BVmult s1, BO_BVmult s2 => N.eqb s1 s2
+   | BO_BVand s1, BO_BVand s2 => N.eqb s1 s2
+   (* | BO_BVor s1, BO_BVor s2  *)
+   (* | BO_BVxor s1, BO_BVxor s2 *)
+   (* | BO_BVadd s1, BO_BVadd s2  *)
+   (* | BO_BVsubst s1, BO_BVsubst s2  *)
+   (* | BO_BVmult s1, BO_BVmult s2 => N.eqb s1 s2 *)
    | _,_ => false
    end.
 
@@ -701,21 +709,21 @@ Module Atom.
 
   Lemma reflect_bop_eqb : forall o1 o2, reflect (o1 = o2) (bop_eqb o1 o2).
   Proof.
-   intros [ | | | | | | | A1|s1|s1 |s1 | s1 | s1 | s1 ] [ | | | | | | | A2|s2|s2| s2 | s2 | s2 | s2 ];simpl;try (constructor;trivial;discriminate).
+   intros [ | | | | | | | A1|s1] [ | | | | | | | A2|s2];simpl;try (constructor;trivial;discriminate).
    - preflect (Typ.reflect_eqb A1 A2).
      constructor;subst;trivial.
    - preflect (N.eqb_spec s1 s2).
      constructor;subst;trivial.
-   - preflect (N.eqb_spec s1 s2).
-     constructor;subst;trivial.
-   - preflect (N.eqb_spec s1 s2).
-     constructor;subst;trivial.
-   - preflect (N.eqb_spec s1 s2).
-     constructor;subst;trivial.
-   - preflect (N.eqb_spec s1 s2).
-     constructor;subst;trivial.
-   - preflect (N.eqb_spec s1 s2).
-     constructor;subst;trivial.
+   (* - preflect (N.eqb_spec s1 s2). *)
+   (*   constructor;subst;trivial. *)
+   (* - preflect (N.eqb_spec s1 s2). *)
+   (*   constructor;subst;trivial. *)
+   (* - preflect (N.eqb_spec s1 s2). *)
+   (*   constructor;subst;trivial. *)
+   (* - preflect (N.eqb_spec s1 s2). *)
+   (*   constructor;subst;trivial. *)
+   (* - preflect (N.eqb_spec s1 s2). *)
+   (*   constructor;subst;trivial. *)
   Qed.
 
   Lemma reflect_nop_eqb : forall o1 o2, reflect (o1 = o2) (nop_eqb o1 o2).
@@ -804,7 +812,7 @@ Module Atom.
         | UO_Zpos => (Typ.Tpositive, Typ.TZ)
         | UO_Zneg => (Typ.Tpositive, Typ.TZ)
         | UO_Zopp => (Typ.TZ, Typ.TZ)
-        | UO_BVbitOf s _ => (Typ.TBV s, Typ.Tbool)
+        | UO_BVbitOf s _ => (Typ.TBV, Typ.Tbool)
   (*      | UO_BVneg s => (Typ.TBV s, Typ.TBV s) *)
         end.
 
@@ -818,12 +826,12 @@ Module Atom.
         | BO_Zge    => ((Typ.TZ,Typ.TZ), Typ.Tbool) 
         | BO_Zgt    => ((Typ.TZ,Typ.TZ), Typ.Tbool)
         | BO_eq t   => ((t,t),Typ.Tbool)
-        | BO_BVand s  => ((Typ.TBV s,Typ.TBV s), Typ.TBV s)
-        | BO_BVor s   => ((Typ.TBV s,Typ.TBV s), Typ.TBV s)
-        | BO_BVxor s   => ((Typ.TBV s,Typ.TBV s), Typ.TBV s)
-        | BO_BVadd s   => ((Typ.TBV s,Typ.TBV s), Typ.TBV s)
-        | BO_BVsubst s   => ((Typ.TBV s,Typ.TBV s), Typ.TBV s)
-        | BO_BVmult s   => ((Typ.TBV s,Typ.TBV s), Typ.TBV s)
+        | BO_BVand s  => ((Typ.TBV,Typ.TBV), Typ.TBV)
+        (* | BO_BVor s   => ((Typ.TBV s,Typ.TBV s), Typ.TBV s) *)
+        (* | BO_BVxor s   => ((Typ.TBV s,Typ.TBV s), Typ.TBV s) *)
+        (* | BO_BVadd s   => ((Typ.TBV s,Typ.TBV s), Typ.TBV s) *)
+        (* | BO_BVsubst s   => ((Typ.TBV s,Typ.TBV s), Typ.TBV s) *)
+        (* | BO_BVmult s   => ((Typ.TBV s,Typ.TBV s), Typ.TBV s) *)
         end.
 
       Definition typ_nop o :=
@@ -936,11 +944,11 @@ Module Atom.
           left. exists Typ.TZ. easy.
           right. intros. rewrite andb_false_r. easy.
 
-         (case (Typ.eqb (get_type h) (Typ.TBV n))).
+         (case (Typ.eqb (get_type h) (Typ.TBV))).
           left. exists Typ.Tbool. easy.
           right. intros. rewrite andb_false_r. easy.
 
-         (case (Typ.eqb (get_type h) (Typ.TBV n))).
+         (case (Typ.eqb (get_type h) (Typ.TBV))).
           left. exists Typ.Tbool. easy.
           right. intros. rewrite andb_false_r. easy.
 
@@ -1000,40 +1008,40 @@ Module Atom.
           right. intros. rewrite andb_false_r. easy.
           right. intros. rewrite andb_false_r. easy.
         (case (Typ.eqb (get_type h1) _)); (case (Typ.eqb (get_type h2) _)).
-          left. exists (Typ.TBV n). rewrite N.eqb_refl. easy.
+          left. exists (Typ.TBV).  easy.
           right. intros. rewrite andb_false_r. easy.
           right. intros. rewrite andb_false_r. easy.
           right. intros. rewrite andb_false_r. easy.
-        (*additional case for BO_BVor*)
-        (case (Typ.eqb (get_type h1) _)); (case (Typ.eqb (get_type h2) _)).
-          left. exists (Typ.TBV n). rewrite N.eqb_refl. easy.
-          right. intros. rewrite andb_false_r. easy.
-          right. intros. rewrite andb_false_r. easy.
-          right. intros. rewrite andb_false_r. easy.
-        (*additional case for BO_BVxor*)
-        (case (Typ.eqb (get_type h1) _)); (case (Typ.eqb (get_type h2) _)).
-          left. exists (Typ.TBV n). rewrite N.eqb_refl. easy.
-          right. intros. rewrite andb_false_r. easy.
-          right. intros. rewrite andb_false_r. easy.
-          right. intros. rewrite andb_false_r. easy.
-        (*additional case for BO_BVadd*)
-        (case (Typ.eqb (get_type h1) _)); (case (Typ.eqb (get_type h2) _)).
-          left. exists (Typ.TBV n). rewrite N.eqb_refl. easy.
-          right. intros. rewrite andb_false_r. easy.
-          right. intros. rewrite andb_false_r. easy.
-          right. intros. rewrite andb_false_r. easy.
-        (*additional case for BO_BVsubst*)
-        (case (Typ.eqb (get_type h1) _)); (case (Typ.eqb (get_type h2) _)).
-          left. exists (Typ.TBV n). rewrite N.eqb_refl. easy.
-          right. intros. rewrite andb_false_r. easy.
-          right. intros. rewrite andb_false_r. easy.
-          right. intros. rewrite andb_false_r. easy.
-        (*additional case for BO_BVmult*)
-        (case (Typ.eqb (get_type h1) _)); (case (Typ.eqb (get_type h2) _)).
-          left. exists (Typ.TBV n). rewrite N.eqb_refl. easy.
-          right. intros. rewrite andb_false_r. easy.
-          right. intros. rewrite andb_false_r. easy.
-          right. intros. rewrite andb_false_r. easy.
+        (* (*additional case for BO_BVor*) *)
+        (* (case (Typ.eqb (get_type h1) _)); (case (Typ.eqb (get_type h2) _)). *)
+        (*   left. exists (Typ.TBV n). rewrite N.eqb_refl. easy. *)
+        (*   right. intros. rewrite andb_false_r. easy. *)
+        (*   right. intros. rewrite andb_false_r. easy. *)
+        (*   right. intros. rewrite andb_false_r. easy. *)
+        (* (*additional case for BO_BVxor*) *)
+        (* (case (Typ.eqb (get_type h1) _)); (case (Typ.eqb (get_type h2) _)). *)
+        (*   left. exists (Typ.TBV n). rewrite N.eqb_refl. easy. *)
+        (*   right. intros. rewrite andb_false_r. easy. *)
+        (*   right. intros. rewrite andb_false_r. easy. *)
+        (*   right. intros. rewrite andb_false_r. easy. *)
+        (* (*additional case for BO_BVadd*) *)
+        (* (case (Typ.eqb (get_type h1) _)); (case (Typ.eqb (get_type h2) _)). *)
+        (*   left. exists (Typ.TBV n). rewrite N.eqb_refl. easy. *)
+        (*   right. intros. rewrite andb_false_r. easy. *)
+        (*   right. intros. rewrite andb_false_r. easy. *)
+        (*   right. intros. rewrite andb_false_r. easy. *)
+        (* (*additional case for BO_BVsubst*) *)
+        (* (case (Typ.eqb (get_type h1) _)); (case (Typ.eqb (get_type h2) _)). *)
+        (*   left. exists (Typ.TBV n). rewrite N.eqb_refl. easy. *)
+        (*   right. intros. rewrite andb_false_r. easy. *)
+        (*   right. intros. rewrite andb_false_r. easy. *)
+        (*   right. intros. rewrite andb_false_r. easy. *)
+        (* (*additional case for BO_BVmult*) *)
+        (* (case (Typ.eqb (get_type h1) _)); (case (Typ.eqb (get_type h2) _)). *)
+        (*   left. exists (Typ.TBV n). rewrite N.eqb_refl. easy. *)
+        (*   right. intros. rewrite andb_false_r. easy. *)
+        (*   right. intros. rewrite andb_false_r. easy. *)
+        (*   right. intros. rewrite andb_false_r. easy. *)
 
         (* N-ary operators *)
         destruct op as [ty]; simpl; case (List.forallb (fun t1 : int => Typ.eqb (get_type t1) ty) ha).
@@ -1101,7 +1109,7 @@ Module Atom.
         | UO_Zpos => apply_unop Typ.Tpositive Typ.TZ Zpos
         | UO_Zneg => apply_unop Typ.Tpositive Typ.TZ Zneg
         | UO_Zopp => apply_unop Typ.TZ Typ.TZ Zopp
-        | UO_BVbitOf s n => apply_unop (Typ.TBV s) Typ.Tbool (@BITVECTOR_LIST.bitOf s n)
+        | UO_BVbitOf s n => apply_unop (Typ.TBV) Typ.Tbool (@BITVECTOR_LIST.bitOf n)
     (*    | UO_BVneg s => apply_unop (Typ.TBV s) (Typ.TBV s)  (@BITVECTOR_LIST.bv_not s) *)
         end.
 
@@ -1115,12 +1123,14 @@ Module Atom.
          | BO_Zge => apply_binop Typ.TZ Typ.TZ Typ.Tbool Zge_bool
          | BO_Zgt => apply_binop Typ.TZ Typ.TZ Typ.Tbool Zgt_bool
          | BO_eq t => apply_binop t t Typ.Tbool (Typ.i_eqb t_i t)
-         | BO_BVand s => apply_binop (Typ.TBV s) (Typ.TBV s) (Typ.TBV s) (@BITVECTOR_LIST.bv_and s)
-         | BO_BVor s  => apply_binop (Typ.TBV s) (Typ.TBV s) (Typ.TBV s) (@BITVECTOR_LIST.bv_or s)
-         | BO_BVxor s  => apply_binop (Typ.TBV s) (Typ.TBV s) (Typ.TBV s) (@BITVECTOR_LIST.bv_xor s)
-         | BO_BVadd s  => apply_binop (Typ.TBV s) (Typ.TBV s) (Typ.TBV s) (@BITVECTOR_LIST.bv_add s)
-         | BO_BVsubst s  => apply_binop (Typ.TBV s) (Typ.TBV s) (Typ.TBV s) (@BITVECTOR_LIST.bv_subst s)
-         | BO_BVmult s  => apply_binop (Typ.TBV s) (Typ.TBV s) (Typ.TBV s) (@BITVECTOR_LIST.bv_mult s)
+         | BO_BVand s =>
+           apply_binop (Typ.TBV) (Typ.TBV) (Typ.TBV) BITVECTOR_LIST.bv_and
+         (* | BO_BVor s  => *)
+         (*   apply_binop (Typ.TBV s) (Typ.TBV s) (Typ.TBV s) BITVECTOR_LIST.bv_or *)
+         (* | BO_BVxor s  => apply_binop (Typ.TBV s) (Typ.TBV s) (Typ.TBV s) (@BITVECTOR_LIST.bv_xor) *)
+         (* | BO_BVadd s  => apply_binop (Typ.TBV s) (Typ.TBV s) (Typ.TBV s) (@BITVECTOR_LIST.bv_add s) *)
+         (* | BO_BVsubst s  => apply_binop (Typ.TBV s) (Typ.TBV s) (Typ.TBV s) (@BITVECTOR_LIST.bv_subst s) *)
+         (* | BO_BVmult s  => apply_binop (Typ.TBV s) (Typ.TBV s) (Typ.TBV s) (@BITVECTOR_LIST.bv_mult s) *)
          end.
 
       Fixpoint compute_interp ty acc l :=
@@ -1237,11 +1247,11 @@ Module Atom.
         | _ => true
         end.
 
-      Definition interp_bv (v:bval) (s:N) : BITVECTOR_LIST.bitvector s :=
+      Definition interp_bv (v:bval) : BITVECTOR_LIST.bitvector :=
         let (t,v) := v in
-        match Typ.cast t (Typ.TBV s) with
+        match Typ.cast t Typ.TBV with
         | Typ.Cast k => k _ v
-        | _ => BITVECTOR_LIST.zeros s
+        | _ => BITVECTOR_LIST.zeros 0
         end.
 
 
@@ -1285,56 +1295,57 @@ Module Atom.
         exists (- y)%Z; auto.
         exists (BITVECTOR_LIST.bitOf n0 y); auto.
         (* Binary operators *)
-        destruct op as [ | | | | | | | A |s1|s2| s3 | s4 | s5 | s6 ]; intros [i | | | |s]; simpl; try discriminate; unfold is_true; rewrite andb_true_iff;
-        try (change (Typ.eqb (get_type h1) Typ.TZ = true /\ Typ.eqb (get_type h2) Typ.TZ = true) with 
-        (is_true (Typ.eqb (get_type h1) Typ.TZ) /\ is_true (Typ.eqb (get_type h2) Typ.TZ)); rewrite !Typ.eqb_spec; intros [H1 H2]; 
-        destruct (check_aux_interp_hatom h1) as [x1 Hx1]; rewrite Hx1; destruct (check_aux_interp_hatom h2) as [x2 Hx2]; 
-        rewrite Hx2; simpl; generalize x1 Hx1 x2 Hx2; rewrite H1, H2; intros y1 Hy1 y2 Hy2; rewrite !Typ.cast_refl);
+Admitted.
+      (*   destruct op as [ | | | | | | | A |s1]; intros [i | | | |s]; simpl; try discriminate; unfold is_true; rewrite andb_true_iff; *)
+      (*   try (change (Typ.eqb (get_type h1) Typ.TZ = true /\ Typ.eqb (get_type h2) Typ.TZ = true) with  *)
+      (*   (is_true (Typ.eqb (get_type h1) Typ.TZ) /\ is_true (Typ.eqb (get_type h2) Typ.TZ)); rewrite !Typ.eqb_spec; intros [H1 H2];  *)
+      (*   destruct (check_aux_interp_hatom h1) as [x1 Hx1]; rewrite Hx1; destruct (check_aux_interp_hatom h2) as [x2 Hx2];  *)
+      (*   rewrite Hx2; simpl; generalize x1 Hx1 x2 Hx2; rewrite H1, H2; intros y1 Hy1 y2 Hy2; rewrite !Typ.cast_refl); *)
 
-        try (change (Typ.eqb (get_type h1) (Typ.TBV s) = true /\ Typ.eqb (get_type h2) (Typ.TBV s) = true) with
-        (is_true (Typ.eqb (get_type h1) (Typ.TBV s)) /\ is_true (Typ.eqb (get_type h2) (Typ.TBV s))); rewrite !Typ.eqb_spec; intros [H1 H2];
-        destruct (check_aux_interp_hatom h1) as [x1 Hx1]; rewrite Hx1; destruct (check_aux_interp_hatom h2) as [x2 Hx2];
-        rewrite Hx2; simpl; generalize x1 Hx1 x2 Hx2; rewrite H1, H2; intros y1 Hy1 y2 Hy2; rewrite !Typ.cast_refl).
+      (*   try (change (Typ.eqb (get_type h1) (Typ.TBV) = true /\ Typ.eqb (get_type h2) (Typ.TBV) = true) with *)
+      (*   (is_true (Typ.eqb (get_type h1) (Typ.TBV)) /\ is_true (Typ.eqb (get_type h2) (Typ.TBV))); rewrite !Typ.eqb_spec; intros [H1 H2]; *)
+      (*   destruct (check_aux_interp_hatom h1) as [x1 Hx1]; rewrite Hx1; destruct (check_aux_interp_hatom h2) as [x2 Hx2]; *)
+      (*   rewrite Hx2; simpl; generalize x1 Hx1 x2 Hx2; rewrite H1, H2; intros y1 Hy1 y2 Hy2; rewrite !Typ.cast_refl). *)
 
-        exists (y1 + y2)%Z; auto.
-        exists (y1 - y2)%Z; auto.
-        exists (y1 * y2)%Z; auto.
-        exists (y1 <? y2)%Z; auto.
-        exists (y1 <=? y2)%Z; auto.
-        exists (y1 >=? y2)%Z; auto.
-        exists (y1 >? y2)%Z; auto.
-        change (Typ.eqb (get_type h1) A = true /\ Typ.eqb (get_type h2) A = true) with (is_true (Typ.eqb (get_type h1) A) /\ is_true (Typ.eqb (get_type h2) A)); rewrite !Typ.eqb_spec; intros [H1 H2]; destruct (check_aux_interp_hatom h1) as [x1 Hx1]; rewrite Hx1; destruct (check_aux_interp_hatom h2) as [x2 Hx2]; rewrite Hx2; simpl; generalize x1 Hx1 x2 Hx2; rewrite H1, H2; intros y1 Hy1 y2 Hy2; rewrite !Typ.cast_refl; exists (Typ.i_eqb t_i A y1 y2); auto.
-        (*BO_BVand*)
-        rewrite andb_true_iff, N.eqb_eq.
-        change ((s1 = s /\ Typ.eqb (get_type h1) (Typ.TBV s1) = true) /\ Typ.eqb (get_type h2) (Typ.TBV s1) = true) with ((s1 = s /\ is_true (Typ.eqb (get_type h1) (Typ.TBV s1))) /\ is_true (Typ.eqb (get_type h2) (Typ.TBV s1))); rewrite !Typ.eqb_spec; intros [[-> H1] H2]; destruct (check_aux_interp_hatom h1) as [x1 Hx1]; rewrite Hx1; destruct (check_aux_interp_hatom h2) as [x2 Hx2]; rewrite Hx2; simpl; generalize x1 Hx1 x2 Hx2; rewrite H1, H2; intros y1 Hy1 y2 Hy2; rewrite !Typ.cast_refl.
-        exists (BITVECTOR_LIST.bv_and y1 y2); auto.   
-        (*BO_BVor*)   
-        rewrite andb_true_iff, N.eqb_eq.
-        change ((s2 = s /\ Typ.eqb (get_type h1) (Typ.TBV s2) = true) /\ Typ.eqb (get_type h2) (Typ.TBV s2) = true) with ((s2 = s /\ is_true (Typ.eqb (get_type h1) (Typ.TBV s2))) /\ is_true (Typ.eqb (get_type h2) (Typ.TBV s2))); rewrite !Typ.eqb_spec; intros [[-> H1] H2]; destruct (check_aux_interp_hatom h1) as [x1 Hx1]; rewrite Hx1; destruct (check_aux_interp_hatom h2) as [x2 Hx2]; rewrite Hx2; simpl; generalize x1 Hx1 x2 Hx2; rewrite H1, H2; intros y1 Hy1 y2 Hy2; rewrite !Typ.cast_refl.
-        exists (BITVECTOR_LIST.bv_or y1 y2); auto.
-        (*BO_BVxor*)   
-        rewrite andb_true_iff, N.eqb_eq.
-        change ((s3 = s /\ Typ.eqb (get_type h1) (Typ.TBV s3) = true) /\ Typ.eqb (get_type h2) (Typ.TBV s3) = true) with ((s3 = s /\ is_true (Typ.eqb (get_type h1) (Typ.TBV s3))) /\ is_true (Typ.eqb (get_type h2) (Typ.TBV s3))); rewrite !Typ.eqb_spec; intros [[-> H1] H2]; destruct (check_aux_interp_hatom h1) as [x1 Hx1]; rewrite Hx1; destruct (check_aux_interp_hatom h2) as [x2 Hx2]; rewrite Hx2; simpl; generalize x1 Hx1 x2 Hx2; rewrite H1, H2; intros y1 Hy1 y2 Hy2; rewrite !Typ.cast_refl.
-        exists (BITVECTOR_LIST.bv_xor y1 y2); auto.
-        (*BO_BVadd*)   
-        rewrite andb_true_iff, N.eqb_eq.
-        change ((s4 = s /\ Typ.eqb (get_type h1) (Typ.TBV s4) = true) /\ Typ.eqb (get_type h2) (Typ.TBV s4) = true) with ((s4 = s /\ is_true (Typ.eqb (get_type h1) (Typ.TBV s4))) /\ is_true (Typ.eqb (get_type h2) (Typ.TBV s4))); rewrite !Typ.eqb_spec; intros [[-> H1] H2]; destruct (check_aux_interp_hatom h1) as [x1 Hx1]; rewrite Hx1; destruct (check_aux_interp_hatom h2) as [x2 Hx2]; rewrite Hx2; simpl; generalize x1 Hx1 x2 Hx2; rewrite H1, H2; intros y1 Hy1 y2 Hy2; rewrite !Typ.cast_refl.
-        exists (BITVECTOR_LIST.bv_add y1 y2); auto. 
-        (*BO_BVsubst*)   
-        rewrite andb_true_iff, N.eqb_eq.
-        change ((s5 = s /\ Typ.eqb (get_type h1) (Typ.TBV s5) = true) /\ Typ.eqb (get_type h2) (Typ.TBV s5) = true) with ((s5 = s /\ is_true (Typ.eqb (get_type h1) (Typ.TBV s5))) /\ is_true (Typ.eqb (get_type h2) (Typ.TBV s5))); rewrite !Typ.eqb_spec; intros [[-> H1] H2]; destruct (check_aux_interp_hatom h1) as [x1 Hx1]; rewrite Hx1; destruct (check_aux_interp_hatom h2) as [x2 Hx2]; rewrite Hx2; simpl; generalize x1 Hx1 x2 Hx2; rewrite H1, H2; intros y1 Hy1 y2 Hy2; rewrite !Typ.cast_refl.
-        exists (BITVECTOR_LIST.bv_subst y1 y2); auto.
-        (*BO_BVmult*)   
-        rewrite andb_true_iff, N.eqb_eq.
-        change ((s6 = s /\ Typ.eqb (get_type h1) (Typ.TBV s6) = true) /\ Typ.eqb (get_type h2) (Typ.TBV s6) = true) with ((s6 = s /\ is_true (Typ.eqb (get_type h1) (Typ.TBV s6))) /\ is_true (Typ.eqb (get_type h2) (Typ.TBV s6))); rewrite !Typ.eqb_spec; intros [[-> H1] H2]; destruct (check_aux_interp_hatom h1) as [x1 Hx1]; rewrite Hx1; destruct (check_aux_interp_hatom h2) as [x2 Hx2]; rewrite Hx2; simpl; generalize x1 Hx1 x2 Hx2; rewrite H1, H2; intros y1 Hy1 y2 Hy2; rewrite !Typ.cast_refl.
-        exists (BITVECTOR_LIST.bv_mult y1 y2); auto.  
-        (* N-ary operators *)
-        destruct op as [A]; simpl; intros [ | | | | ]; try discriminate; simpl; intros _; case (compute_interp A nil ha).
-        intro l; exists (distinct (Typ.i_eqb t_i A) (rev l)); auto.
-        exists true; auto.
-        (* Application *)
-        intro t; apply check_args_interp_aux.
-      Qed.
+      (*   exists (y1 + y2)%Z; auto. *)
+      (*   exists (y1 - y2)%Z; auto. *)
+      (*   exists (y1 * y2)%Z; auto. *)
+      (*   exists (y1 <? y2)%Z; auto. *)
+      (*   exists (y1 <=? y2)%Z; auto. *)
+      (*   exists (y1 >=? y2)%Z; auto. *)
+      (*   exists (y1 >? y2)%Z; auto. *)
+      (*   change (Typ.eqb (get_type h1) A = true /\ Typ.eqb (get_type h2) A = true) with (is_true (Typ.eqb (get_type h1) A) /\ is_true (Typ.eqb (get_type h2) A)); rewrite !Typ.eqb_spec; intros [H1 H2]; destruct (check_aux_interp_hatom h1) as [x1 Hx1]; rewrite Hx1; destruct (check_aux_interp_hatom h2) as [x2 Hx2]; rewrite Hx2; simpl; generalize x1 Hx1 x2 Hx2; rewrite H1, H2; intros y1 Hy1 y2 Hy2; rewrite !Typ.cast_refl; exists (Typ.i_eqb t_i A y1 y2); auto. *)
+      (*   (*BO_BVand*) *)
+      (*   rewrite andb_true_iff, N.eqb_eq. *)
+      (*   change ((s1 = s /\ Typ.eqb (get_type h1) (Typ.TBV1) = true) /\ Typ.eqb (get_type h2) (Typ.TBV1) = true) with ((s1 = s /\ is_true (Typ.eqb (get_type h1) (Typ.TBV1))) /\ is_true (Typ.eqb (get_type h2) (Typ.TBV1))); rewrite !Typ.eqb_spec; intros [[-> H1] H2]; destruct (check_aux_interp_hatom h1) as [x1 Hx1]; rewrite Hx1; destruct (check_aux_interp_hatom h2) as [x2 Hx2]; rewrite Hx2; simpl; generalize x1 Hx1 x2 Hx2; rewrite H1, H2; intros y1 Hy1 y2 Hy2; rewrite !Typ.cast_refl. *)
+      (*   exists (BITVECTOR_LIST.bv_and y1 y2); auto.    *)
+      (*   (*BO_BVor*)    *)
+      (*   rewrite andb_true_iff, N.eqb_eq. *)
+      (*   change ((s2 = s /\ Typ.eqb (get_type h1) (Typ.TBV2) = true) /\ Typ.eqb (get_type h2) (Typ.TBV2) = true) with ((s2 = s /\ is_true (Typ.eqb (get_type h1) (Typ.TBV2))) /\ is_true (Typ.eqb (get_type h2) (Typ.TBV2))); rewrite !Typ.eqb_spec; intros [[-> H1] H2]; destruct (check_aux_interp_hatom h1) as [x1 Hx1]; rewrite Hx1; destruct (check_aux_interp_hatom h2) as [x2 Hx2]; rewrite Hx2; simpl; generalize x1 Hx1 x2 Hx2; rewrite H1, H2; intros y1 Hy1 y2 Hy2; rewrite !Typ.cast_refl. *)
+      (*   exists (BITVECTOR_LIST.bv_or y1 y2); auto. *)
+      (*   (*BO_BVxor*)    *)
+      (*   rewrite andb_true_iff, N.eqb_eq. *)
+      (*   change ((s3 = s /\ Typ.eqb (get_type h1) (Typ.TBV3) = true) /\ Typ.eqb (get_type h2) (Typ.TBV3) = true) with ((s3 = s /\ is_true (Typ.eqb (get_type h1) (Typ.TBV3))) /\ is_true (Typ.eqb (get_type h2) (Typ.TBV3))); rewrite !Typ.eqb_spec; intros [[-> H1] H2]; destruct (check_aux_interp_hatom h1) as [x1 Hx1]; rewrite Hx1; destruct (check_aux_interp_hatom h2) as [x2 Hx2]; rewrite Hx2; simpl; generalize x1 Hx1 x2 Hx2; rewrite H1, H2; intros y1 Hy1 y2 Hy2; rewrite !Typ.cast_refl. *)
+      (*   exists (BITVECTOR_LIST.bv_xor y1 y2); auto. *)
+      (*   (*BO_BVadd*)    *)
+      (*   rewrite andb_true_iff, N.eqb_eq. *)
+      (*   change ((s4 = s /\ Typ.eqb (get_type h1) (Typ.TBV4) = true) /\ Typ.eqb (get_type h2) (Typ.TBV4) = true) with ((s4 = s /\ is_true (Typ.eqb (get_type h1) (Typ.TBV4))) /\ is_true (Typ.eqb (get_type h2) (Typ.TBV4))); rewrite !Typ.eqb_spec; intros [[-> H1] H2]; destruct (check_aux_interp_hatom h1) as [x1 Hx1]; rewrite Hx1; destruct (check_aux_interp_hatom h2) as [x2 Hx2]; rewrite Hx2; simpl; generalize x1 Hx1 x2 Hx2; rewrite H1, H2; intros y1 Hy1 y2 Hy2; rewrite !Typ.cast_refl. *)
+      (*   exists (BITVECTOR_LIST.bv_add y1 y2); auto.  *)
+      (*   (*BO_BVsubst*)    *)
+      (*   rewrite andb_true_iff, N.eqb_eq. *)
+      (*   change ((s5 = s /\ Typ.eqb (get_type h1) (Typ.TBV5) = true) /\ Typ.eqb (get_type h2) (Typ.TBV5) = true) with ((s5 = s /\ is_true (Typ.eqb (get_type h1) (Typ.TBV5))) /\ is_true (Typ.eqb (get_type h2) (Typ.TBV5))); rewrite !Typ.eqb_spec; intros [[-> H1] H2]; destruct (check_aux_interp_hatom h1) as [x1 Hx1]; rewrite Hx1; destruct (check_aux_interp_hatom h2) as [x2 Hx2]; rewrite Hx2; simpl; generalize x1 Hx1 x2 Hx2; rewrite H1, H2; intros y1 Hy1 y2 Hy2; rewrite !Typ.cast_refl. *)
+      (*   exists (BITVECTOR_LIST.bv_subst y1 y2); auto. *)
+      (*   (*BO_BVmult*)    *)
+      (*   rewrite andb_true_iff, N.eqb_eq. *)
+      (*   change ((s6 = s /\ Typ.eqb (get_type h1) (Typ.TBV6) = true) /\ Typ.eqb (get_type h2) (Typ.TBV6) = true) with ((s6 = s /\ is_true (Typ.eqb (get_type h1) (Typ.TBV6))) /\ is_true (Typ.eqb (get_type h2) (Typ.TBV6))); rewrite !Typ.eqb_spec; intros [[-> H1] H2]; destruct (check_aux_interp_hatom h1) as [x1 Hx1]; rewrite Hx1; destruct (check_aux_interp_hatom h2) as [x2 Hx2]; rewrite Hx2; simpl; generalize x1 Hx1 x2 Hx2; rewrite H1, H2; intros y1 Hy1 y2 Hy2; rewrite !Typ.cast_refl. *)
+      (*   exists (BITVECTOR_LIST.bv_mult y1 y2); auto.   *)
+      (*   (* N-ary operators *) *)
+      (*   destruct op as [A]; simpl; intros [ | | | | ]; try discriminate; simpl; intros _; case (compute_interp A nil ha). *)
+      (*   intro l; exists (distinct (Typ.i_eqb t_i A) (rev l)); auto. *)
+      (*   exists true; auto. *)
+      (*   (* Application *) *)
+      (*   intro t; apply check_args_interp_aux. *)
+      (* Qed. *)
 
       (* If an atom is not well-typed, its interpretation is bvtrue *)
 
@@ -1365,22 +1376,23 @@ Module Atom.
         (* Unary operators *)
         destruct op; simpl; intro H; destruct (check_aux_interp_hatom h) as [v Hv]; rewrite Hv; simpl; rewrite Typ.neq_cast; try (pose (H2 := H Typ.Tpositive); simpl in H2; rewrite H2; auto); try (pose (H2 := H Typ.TZ); simpl in H2; rewrite H2; auto); pose (H2 := H Typ.Tbool); simpl in H2; rewrite H2; auto.
         (* Binary operators *)
-        destruct op; simpl; intro H; destruct (check_aux_interp_hatom h1) as [v1 Hv1]; destruct (check_aux_interp_hatom h2) as [v2 Hv2]; rewrite Hv1, Hv2; simpl;
- try (pose (H2 := H Typ.TZ); simpl in H2; rewrite andb_false_iff in H2; destruct H2 as [H2|H2]; [rewrite (Typ.neq_cast (get_type h1)), H2|rewrite (Typ.neq_cast (get_type h2)), H2; case (Typ.cast (get_type h1) Typ.TZ)]; auto);
- try (pose (H2 := H Typ.Tbool); simpl in H2; rewrite andb_false_iff in H2; destruct H2 as [H2|H2]; [rewrite (Typ.neq_cast (get_type h1)), H2|rewrite (Typ.neq_cast (get_type h2)), H2; case (Typ.cast (get_type h1) Typ.TZ)]; auto);
- try (pose (H2 := H (Typ.TBV n)); simpl in H2; rewrite !andb_false_iff in H2; destruct H2 as [[H2|H2]|H2]; [rewrite N.eqb_refl in H2; discriminate | rewrite (Typ.neq_cast (get_type h1)), H2|rewrite (Typ.neq_cast (get_type h2)), H2; case (Typ.cast (get_type h1) (Typ.TBV n)); case (Typ.cast (get_type h1) (Typ.TBV n))]; auto);
- case (Typ.cast (get_type h1) t); auto.
-        (* N-ary operators *)
-        destruct op as [A]; simpl; intro H; generalize (H Typ.Tbool); simpl; clear H; assert (H: forall l1, List.forallb (fun t1 : int => Typ.eqb (get_type t1) A) ha = false -> match compute_interp A l1 ha with | Some l => Bval Typ.Tbool (distinct (Typ.i_eqb t_i A) (rev l)) | None => bvtrue end = bvtrue).
-        induction ha as [ |h ha Iha]; simpl.
-        intros; discriminate.
-        intro l1; destruct (check_aux_interp_hatom h) as [vh Hh]; case_eq (Typ.eqb (get_type h) A); simpl.
-        change (Typ.eqb (get_type h) A = true) with (is_true (Typ.eqb (get_type h) A)); rewrite Typ.eqb_spec; intro; subst A; intro H; rewrite Hh; simpl; rewrite Typ.cast_refl; apply Iha; auto.
-        intros H _; rewrite Hh; simpl; rewrite (Typ.cast_diff _ _ H); auto.
-        apply H.
-        (* Application *)
-        apply check_args_interp_aux_contr.
-      Qed.
+        Admitted.
+ (*        destruct op; simpl; intro H; destruct (check_aux_interp_hatom h1) as [v1 Hv1]; destruct (check_aux_interp_hatom h2) as [v2 Hv2]; rewrite Hv1, Hv2; simpl; *)
+ (* try (pose (H2 := H Typ.TZ); simpl in H2; rewrite andb_false_iff in H2; destruct H2 as [H2|H2]; [rewrite (Typ.neq_cast (get_type h1)), H2|rewrite (Typ.neq_cast (get_type h2)), H2; case (Typ.cast (get_type h1) Typ.TZ)]; auto); *)
+ (* try (pose (H2 := H Typ.Tbool); simpl in H2; rewrite andb_false_iff in H2; destruct H2 as [H2|H2]; [rewrite (Typ.neq_cast (get_type h1)), H2|rewrite (Typ.neq_cast (get_type h2)), H2; case (Typ.cast (get_type h1) Typ.TZ)]; auto); *)
+ (* try (pose (H2 := H (Typ.TBV)); simpl in H2; rewrite !andb_false_iff in H2; destruct H2 as [[H2|H2]|H2]; [rewrite N.eqb_refl in H2; discriminate | rewrite (Typ.neq_cast (get_type h1)), H2|rewrite (Typ.neq_cast (get_type h2)), H2; case (Typ.cast (get_type h1) (Typ.TBV)); case (Typ.cast (get_type h1) (Typ.TBV))]; auto); *)
+ (* case (Typ.cast (get_type h1) t); auto. *)
+ (*        (* N-ary operators *) *)
+ (*        destruct op as [A]; simpl; intro H; generalize (H Typ.Tbool); simpl; clear H; assert (H: forall l1, List.forallb (fun t1 : int => Typ.eqb (get_type t1) A) ha = false -> match compute_interp A l1 ha with | Some l => Bval Typ.Tbool (distinct (Typ.i_eqb t_i A) (rev l)) | None => bvtrue end = bvtrue). *)
+ (*        induction ha as [ |h ha Iha]; simpl. *)
+ (*        intros; discriminate. *)
+ (*        intro l1; destruct (check_aux_interp_hatom h) as [vh Hh]; case_eq (Typ.eqb (get_type h) A); simpl. *)
+ (*        change (Typ.eqb (get_type h) A = true) with (is_true (Typ.eqb (get_type h) A)); rewrite Typ.eqb_spec; intro; subst A; intro H; rewrite Hh; simpl; rewrite Typ.cast_refl; apply Iha; auto. *)
+ (*        intros H _; rewrite Hh; simpl; rewrite (Typ.cast_diff _ _ H); auto. *)
+ (*        apply H. *)
+ (*        (* Application *) *)
+ (*        apply check_args_interp_aux_contr. *)
+ (*      Qed. *)
 
     End Interp_Aux.
 
@@ -1537,36 +1549,37 @@ Module Atom.
         case (Typ.cast (v_type Typ.type interp_t (a .[ i])) Typ.Tpositive); simpl; try (exists true; auto); intro k; exists (Zpos (k interp_t x)); auto.
         case (Typ.cast (v_type Typ.type interp_t (a .[ i])) Typ.Tpositive); simpl; try (exists true; auto); intro k; exists (Zneg (k interp_t x)); auto.
         case (Typ.cast (v_type Typ.type interp_t (a .[ i])) Typ.TZ); simpl; try (exists true; auto); intro k; exists (- k interp_t x)%Z; auto.
-        case (Typ.cast (v_type Typ.type interp_t (a .[ i])) (Typ.TBV n)); simpl; [ | exists true; auto]. intro k; exists (BITVECTOR_LIST.bitOf n0 (k interp_t x)) ; auto.
+        case (Typ.cast (v_type Typ.type interp_t (a .[ i])) (Typ.TBV)); simpl; [ | exists true; auto]. intro k; exists (BITVECTOR_LIST.bitOf n0 (k interp_t x)) ; auto.
         (* Binary operators *)
-        intros [ | | | | | | |A | | | | | | ] h1 h2; simpl; rewrite andb_true_iff; intros [H1 H2]; destruct (IH h1 H1) as [x Hx]; destruct (IH h2 H2) as [y Hy]; rewrite Hx, Hy; simpl.
-        case (Typ.cast (v_type Typ.type interp_t (a .[ h1])) Typ.TZ); simpl; try (exists true; auto); intro k1; case (Typ.cast (v_type Typ.type interp_t (a .[ h2])) Typ.TZ); simpl; try (exists true; auto); intro k2; exists (k1 interp_t x + k2 interp_t y)%Z; auto.
-        case (Typ.cast (v_type Typ.type interp_t (a .[ h1])) Typ.TZ); simpl; try (exists true; auto); intro k1; case (Typ.cast (v_type Typ.type interp_t (a .[ h2])) Typ.TZ); simpl; try (exists true; auto); intro k2; exists (k1 interp_t x - k2 interp_t y)%Z; auto.
-        case (Typ.cast (v_type Typ.type interp_t (a .[ h1])) Typ.TZ); simpl; try (exists true; auto); intro k1; case (Typ.cast (v_type Typ.type interp_t (a .[ h2])) Typ.TZ); simpl; try (exists true; auto); intro k2; exists (k1 interp_t x * k2 interp_t y)%Z; auto.
-        case (Typ.cast (v_type Typ.type interp_t (a .[ h1])) Typ.TZ); simpl; try (exists true; auto); intro k1; case (Typ.cast (v_type Typ.type interp_t (a .[ h2])) Typ.TZ) as [k2| ]; simpl; try (exists true; reflexivity); exists (k1 interp_t x <? k2 interp_t y); auto.
-        case (Typ.cast (v_type Typ.type interp_t (a .[ h1])) Typ.TZ); simpl; try (exists true; auto); intro k1; case (Typ.cast (v_type Typ.type interp_t (a .[ h2])) Typ.TZ) as [k2| ]; simpl; try (exists true; reflexivity); exists (k1 interp_t x <=? k2 interp_t y); auto.
-        case (Typ.cast (v_type Typ.type interp_t (a .[ h1])) Typ.TZ); simpl; try (exists true; auto); intro k1; case (Typ.cast (v_type Typ.type interp_t (a .[ h2])) Typ.TZ) as [k2| ]; simpl; try (exists true; reflexivity); exists (k1 interp_t x >=? k2 interp_t y); auto.
-        case (Typ.cast (v_type Typ.type interp_t (a .[ h1])) Typ.TZ); simpl; try (exists true; auto); intro k1; case (Typ.cast (v_type Typ.type interp_t (a .[ h2])) Typ.TZ) as [k2| ]; simpl; try (exists true; reflexivity); exists (k1 interp_t x >? k2 interp_t y); auto.
-        case (Typ.cast (v_type Typ.type interp_t (a .[ h1])) A); simpl; try (exists true; auto); intro k1; case (Typ.cast (v_type Typ.type interp_t (a .[ h2])) A) as [k2| ]; simpl; try (exists true; reflexivity); exists (Typ.i_eqb t_i A (k1 interp_t x) (k2 interp_t y)); auto.
-        (*BO_BVand*)
-        case (Typ.cast (v_type Typ.type interp_t (a .[ h1])) (Typ.TBV n)); simpl; try (exists true; auto); intro k1; case (Typ.cast (v_type Typ.type interp_t (a .[ h2])) (Typ.TBV n)) as [k2| ]; simpl; try (exists true; reflexivity); exists (BITVECTOR_LIST.bv_and (k1 interp_t x) (k2 interp_t y)); auto.
-        (*BO_BVor*)
-        case (Typ.cast (v_type Typ.type interp_t (a .[ h1])) (Typ.TBV n)); simpl; try (exists true; auto); intro k1; case (Typ.cast (v_type Typ.type interp_t (a .[ h2])) (Typ.TBV n)) as [k2| ]; simpl; try (exists true; reflexivity); exists (BITVECTOR_LIST.bv_or (k1 interp_t x) (k2 interp_t y)); auto.        
-        (*BO_BVxor*)
-        case (Typ.cast (v_type Typ.type interp_t (a .[ h1])) (Typ.TBV n)); simpl; try (exists true; auto); intro k1; case (Typ.cast (v_type Typ.type interp_t (a .[ h2])) (Typ.TBV n)) as [k2| ]; simpl; try (exists true; reflexivity); exists (BITVECTOR_LIST.bv_xor (k1 interp_t x) (k2 interp_t y)); auto.        
-        (*BO_BVadd*)
-        case (Typ.cast (v_type Typ.type interp_t (a .[ h1])) (Typ.TBV n)); simpl; try (exists true; auto); intro k1; case (Typ.cast (v_type Typ.type interp_t (a .[ h2])) (Typ.TBV n)) as [k2| ]; simpl; try (exists true; reflexivity); exists (BITVECTOR_LIST.bv_add (k1 interp_t x) (k2 interp_t y)); auto.    
-        (*BO_BVsubst*)
-        case (Typ.cast (v_type Typ.type interp_t (a .[ h1])) (Typ.TBV n)); simpl; try (exists true; auto); intro k1; case (Typ.cast (v_type Typ.type interp_t (a .[ h2])) (Typ.TBV n)) as [k2| ]; simpl; try (exists true; reflexivity); exists (BITVECTOR_LIST.bv_subst (k1 interp_t x) (k2 interp_t y)); auto.
-        (*BO_BVmult*)
-        case (Typ.cast (v_type Typ.type interp_t (a .[ h1])) (Typ.TBV n)); simpl; try (exists true; auto); intro k1; case (Typ.cast (v_type Typ.type interp_t (a .[ h2])) (Typ.TBV n)) as [k2| ]; simpl; try (exists true; reflexivity); exists (BITVECTOR_LIST.bv_mult (k1 interp_t x) (k2 interp_t y)); auto.
-        (* N-ary operators *)       
-        intros [A] l; assert (forall acc, List.forallb (fun h0 : int => h0 < h) l = true -> exists v, match compute_interp (get a) A acc l with | Some l0 => Bval Typ.Tbool (distinct (Typ.i_eqb t_i A) (rev l0)) | None => bvtrue end = Bval (v_type Typ.type interp_t match compute_interp (get a) A acc l with | Some l0 => Bval Typ.Tbool (distinct (Typ.i_eqb t_i A) (rev l0)) | None => bvtrue end) v); auto; induction l as [ |i l IHl]; simpl.
-        intros acc _; exists (distinct (Typ.i_eqb t_i A) (rev acc)); auto.
-        intro acc; rewrite andb_true_iff; intros [H1 H2]; destruct (IH _ H1) as [va Hva]; rewrite Hva; simpl; case (Typ.cast (v_type Typ.type interp_t (a .[ i])) A); simpl; try (exists true; auto); intro k; destruct (IHl (k interp_t va :: acc) H2) as [vb Hvb]; exists vb; auto.
-        (* Application *)
-        intros i l H; apply (check_aux_interp_aux_lt_aux a h IH l H (t_func.[i])).
-      Qed.
+        Admitted.
+      (*   intros [ | | | | | | |A | | | | | | ] h1 h2; simpl; rewrite andb_true_iff; intros [H1 H2]; destruct (IH h1 H1) as [x Hx]; destruct (IH h2 H2) as [y Hy]; rewrite Hx, Hy; simpl. *)
+      (*   case (Typ.cast (v_type Typ.type interp_t (a .[ h1])) Typ.TZ); simpl; try (exists true; auto); intro k1; case (Typ.cast (v_type Typ.type interp_t (a .[ h2])) Typ.TZ); simpl; try (exists true; auto); intro k2; exists (k1 interp_t x + k2 interp_t y)%Z; auto. *)
+      (*   case (Typ.cast (v_type Typ.type interp_t (a .[ h1])) Typ.TZ); simpl; try (exists true; auto); intro k1; case (Typ.cast (v_type Typ.type interp_t (a .[ h2])) Typ.TZ); simpl; try (exists true; auto); intro k2; exists (k1 interp_t x - k2 interp_t y)%Z; auto. *)
+      (*   case (Typ.cast (v_type Typ.type interp_t (a .[ h1])) Typ.TZ); simpl; try (exists true; auto); intro k1; case (Typ.cast (v_type Typ.type interp_t (a .[ h2])) Typ.TZ); simpl; try (exists true; auto); intro k2; exists (k1 interp_t x * k2 interp_t y)%Z; auto. *)
+      (*   case (Typ.cast (v_type Typ.type interp_t (a .[ h1])) Typ.TZ); simpl; try (exists true; auto); intro k1; case (Typ.cast (v_type Typ.type interp_t (a .[ h2])) Typ.TZ) as [k2| ]; simpl; try (exists true; reflexivity); exists (k1 interp_t x <? k2 interp_t y); auto. *)
+      (*   case (Typ.cast (v_type Typ.type interp_t (a .[ h1])) Typ.TZ); simpl; try (exists true; auto); intro k1; case (Typ.cast (v_type Typ.type interp_t (a .[ h2])) Typ.TZ) as [k2| ]; simpl; try (exists true; reflexivity); exists (k1 interp_t x <=? k2 interp_t y); auto. *)
+      (*   case (Typ.cast (v_type Typ.type interp_t (a .[ h1])) Typ.TZ); simpl; try (exists true; auto); intro k1; case (Typ.cast (v_type Typ.type interp_t (a .[ h2])) Typ.TZ) as [k2| ]; simpl; try (exists true; reflexivity); exists (k1 interp_t x >=? k2 interp_t y); auto. *)
+      (*   case (Typ.cast (v_type Typ.type interp_t (a .[ h1])) Typ.TZ); simpl; try (exists true; auto); intro k1; case (Typ.cast (v_type Typ.type interp_t (a .[ h2])) Typ.TZ) as [k2| ]; simpl; try (exists true; reflexivity); exists (k1 interp_t x >? k2 interp_t y); auto. *)
+      (*   case (Typ.cast (v_type Typ.type interp_t (a .[ h1])) A); simpl; try (exists true; auto); intro k1; case (Typ.cast (v_type Typ.type interp_t (a .[ h2])) A) as [k2| ]; simpl; try (exists true; reflexivity); exists (Typ.i_eqb t_i A (k1 interp_t x) (k2 interp_t y)); auto. *)
+      (*   (*BO_BVand*) *)
+      (*   case (Typ.cast (v_type Typ.type interp_t (a .[ h1])) (Typ.TBV)); simpl; try (exists true; auto); intro k1; case (Typ.cast (v_type Typ.type interp_t (a .[ h2])) (Typ.TBV)) as [k2| ]; simpl; try (exists true; reflexivity); exists (BITVECTOR_LIST.bv_and (k1 interp_t x) (k2 interp_t y)); auto. *)
+      (*   (* (*BO_BVor*) *) *)
+      (*   (* case (Typ.cast (v_type Typ.type interp_t (a .[ h1])) (Typ.TBV)); simpl; try (exists true; auto); intro k1; case (Typ.cast (v_type Typ.type interp_t (a .[ h2])) (Typ.TBV)) as [k2| ]; simpl; try (exists true; reflexivity); exists (BITVECTOR_LIST.bv_or (k1 interp_t x) (k2 interp_t y)); auto.         *) *)
+      (*   (* (*BO_BVxor*) *) *)
+      (*   (* case (Typ.cast (v_type Typ.type interp_t (a .[ h1])) (Typ.TBV)); simpl; try (exists true; auto); intro k1; case (Typ.cast (v_type Typ.type interp_t (a .[ h2])) (Typ.TBV)) as [k2| ]; simpl; try (exists true; reflexivity); exists (BITVECTOR_LIST.bv_xor (k1 interp_t x) (k2 interp_t y)); auto.         *) *)
+      (*   (* (*BO_BVadd*) *) *)
+      (*   (* case (Typ.cast (v_type Typ.type interp_t (a .[ h1])) (Typ.TBV)); simpl; try (exists true; auto); intro k1; case (Typ.cast (v_type Typ.type interp_t (a .[ h2])) (Typ.TBV)) as [k2| ]; simpl; try (exists true; reflexivity); exists (BITVECTOR_LIST.bv_add (k1 interp_t x) (k2 interp_t y)); auto.     *) *)
+      (*   (* (*BO_BVsubst*) *) *)
+      (*   (* case (Typ.cast (v_type Typ.type interp_t (a .[ h1])) (Typ.TBV)); simpl; try (exists true; auto); intro k1; case (Typ.cast (v_type Typ.type interp_t (a .[ h2])) (Typ.TBV)) as [k2| ]; simpl; try (exists true; reflexivity); exists (BITVECTOR_LIST.bv_subst (k1 interp_t x) (k2 interp_t y)); auto. *) *)
+      (*   (* (*BO_BVmult*) *) *)
+      (*   (* case (Typ.cast (v_type Typ.type interp_t (a .[ h1])) (Typ.TBV)); simpl; try (exists true; auto); intro k1; case (Typ.cast (v_type Typ.type interp_t (a .[ h2])) (Typ.TBV)) as [k2| ]; simpl; try (exists true; reflexivity); exists (BITVECTOR_LIST.bv_mult (k1 interp_t x) (k2 interp_t y)); auto. *) *)
+      (*   (* N-ary operators *)        *)
+      (*   intros [A] l; assert (forall acc, List.forallb (fun h0 : int => h0 < h) l = true -> exists v, match compute_interp (get a) A acc l with | Some l0 => Bval Typ.Tbool (distinct (Typ.i_eqb t_i A) (rev l0)) | None => bvtrue end = Bval (v_type Typ.type interp_t match compute_interp (get a) A acc l with | Some l0 => Bval Typ.Tbool (distinct (Typ.i_eqb t_i A) (rev l0)) | None => bvtrue end) v); auto; induction l as [ |i l IHl]; simpl. *)
+      (*   intros acc _; exists (distinct (Typ.i_eqb t_i A) (rev acc)); auto. *)
+      (*   intro acc; rewrite andb_true_iff; intros [H1 H2]; destruct (IH _ H1) as [va Hva]; rewrite Hva; simpl; case (Typ.cast (v_type Typ.type interp_t (a .[ i])) A); simpl; try (exists true; auto); intro k; destruct (IHl (k interp_t va :: acc) H2) as [vb Hvb]; exists vb; auto. *)
+      (*   (* Application *) *)
+      (*   intros i l H; apply (check_aux_interp_aux_lt_aux a h IH l H (t_func.[i])). *)
+      (* Qed. *)
 
       Lemma check_aux_interp_hatom_lt : forall h, h < length t_atom ->
         exists v, t_interp.[h] = Bval (get_type h) v.
@@ -1639,9 +1652,9 @@ Module Atom.
       fun a => interp_bool (interp a).
 
     Definition interp_form_hatom_bv t_atom :
-      hatom -> forall s, BITVECTOR_LIST.bitvector s :=
+      hatom -> BITVECTOR_LIST.bitvector :=
       let interp := interp_hatom t_atom in
-      fun a s => interp_bv (interp a) s.
+      fun a => interp_bv (interp a).
 
   End Typing_Interp.
 
